default siek cc + simulation with trnslation into dyn language + taut example

theories/dyn_lang/casts.v
@@ -16,6 +16,12 @@ Section casts.
     | Opposite => Normal
     end.
 
+  Definition comp (dir : direction) (f1 f2 : val) :=
+    match dir with
+    | Normal => LamV (AppAn (of_val f2).[ren (+1)] (AppAn (of_val f1).[ren (+1)] (Var 0)))
+    | Opposite => LamV (AppAn (of_val f1).[ren (+1)] (AppAn (of_val f2).[ren (+1)] (Var 0)))
+    end.
+
   Fixpoint cast_upwards (ℓ : label) (τ : type) (dir : direction) : val :=
     match τ with
     | Base B => match dir with
@@ -26,25 +32,24 @@ Section casts.
         match decide (τ1 = Unknown ∧ τ2 = Unknown) with
         | left x => match dir with
                    | Normal => (* ? ∘ ? => ? *) Id
-                   | Opposite => (* ? => ? ∘ ? *) of_shape ℓ (S_Bin bin)
+                   | Opposite => (* ? => ? ∘ ? *) of_shape' ℓ (S_Bin bin)
                    end
-        | right x => (match bin with
-                     | Arrow => surround
-                     | Sum => bimap_sum
-                     | Product => bimap_prod
-                     end)
-                      (match dir with
-                       | Normal => ν
-                       | Opposite => ℓ
-                       end)
-                      (cast_upwards ℓ τ1 (match bin with
-                                          | Arrow => switch (dir)
-                                          | _ => dir
-                                          end)) (cast_upwards ℓ τ2 dir)
+        | right x => comp dir
+                     (match bin with
+                      | Arrow => surround ν
+                      | Sum => bimap_sum ν
+                      | Product => bimap_prod ν
+                      end
+                       (cast_upwards ℓ τ1 (match bin with | Arrow => switch (dir) | _ => dir end))
+                       (cast_upwards ℓ τ2 dir)
+                     )
+                     (match dir with
+                      | Normal => Id
+                      | Opposite => of_shape' ℓ (S_Bin bin)
+                      end)
         end
     | Unknown => Id
     end.
-
 
   Fixpoint cast_pre (ℓ : label) τ τ' (H : consistency τ τ') (dir : direction) : val :=
     match H with
@@ -72,7 +77,7 @@ Section casts.
     induction τ; intros; intro σ; asimpl.
     - destruct dir, B; auto.
     - destruct (decide ((τ1 = Unknown) ∧ (τ2 = Unknown))) as [[-> ->] | bbb].
-      + by destruct dir, bin; asimpl.
+      + destruct dir, bin; asimpl; try done.
       + destruct bin, dir; asimpl; repeat rewrite IHτ1 IHτ2; auto.
     - auto.
   Qed.
@@ -95,11 +100,42 @@ Section casts_alt.
 
   Context {ν : label} {Hν : NeverOccurs ν}.
 
+  Lemma cast_pre_const_rw (ℓ : label) τ τ' (H : consistency τ τ') :
+    ∀ H' dir, cast_pre ℓ τ τ' H dir = cast_pre ℓ τ τ' H' dir.
+  Proof.
+    induction H; intros.
+    - dependent destruction H'; auto.
+    - dependent destruction H'; auto.
+    - dependent destruction H'; auto.
+    - dependent destruction H'; auto.
+      simpl. destruct bin; (f_equiv; [ apply IHconsistency1 | apply IHconsistency2 ]).
+  Qed.
+
+  Lemma cast_pre_sym ℓ τ τ' (H : consistency τ τ') :
+    ∀ dir (H' : consistency τ' τ), cast_pre ℓ τ τ' H dir = cast_pre ℓ τ' τ H' (switch dir).
+  Proof.
+    induction H; intros.
+    - dependent destruction H'; simpl; auto.
+      destruct dir; auto.
+    - dependent destruction H'; simpl; auto.
+    - dependent destruction H'; simpl; auto.
+    - dependent destruction H'; simpl; auto;
+      destruct bin; auto.
+      + f_equiv.
+        apply IHconsistency1.
+        apply IHconsistency2.
+      + f_equiv.
+        apply IHconsistency1.
+        apply IHconsistency2.
+      + f_equiv.
+        apply IHconsistency1.
+        apply IHconsistency2.
+  Qed.
+
   Definition cast' ℓ τ τ' := (match consistency_decision τ τ' with
                               | inl p => cast ℓ τ τ' p
                               | inr _ => LitV LitUnit
                               end).
-
 
   Lemma cast'_closed ℓ τ1 τ2 : Closed (of_val $ cast' ℓ τ1 τ2).
   Proof. rewrite /cast'. destruct (consistency_decision τ1 τ2). apply cast_closed. by asimpl. Qed.
@@ -122,4 +158,155 @@ Section casts_alt.
     dependent destruction c; auto.
   Qed.
 
+  Lemma cast_U_rw ℓ :
+    cast' ℓ Unknown Unknown = Id.
+  Proof.
+    rewrite /cast'.
+    destruct (consistency_decision Unknown Unknown) as [C | nC] eqn:eq.
+    2: { exfalso. apply nC. by constructor. }
+    rewrite /cast /=. by dependent destruction C.
+  Qed.
+
+  Lemma cast_B_rw ℓ B :
+    cast' ℓ (Base B) (Base B) = Id.
+  Proof.
+    rewrite /cast'.
+    destruct (consistency_decision (Base B) (Base B)) as [C | nC] eqn:eq.
+    2: { exfalso. apply nC. by constructor. }
+    rewrite /cast /=. by dependent destruction C.
+  Qed.
+
+  Lemma cast_arrow_rw ℓ τ1 τ2 τ3 τ4 (H13 : consistency τ1 τ3) (H24: consistency τ2 τ4) :
+    cast' ℓ (Bin Arrow τ1 τ2) (Bin Arrow τ3 τ4) =
+    surround ν (cast' ℓ τ3 τ1) (cast' ℓ τ2 τ4).
+  Proof.
+    rewrite /(cast' ℓ (Bin Arrow τ1 τ2) (Bin Arrow τ3 τ4)).
+    destruct (consistency_decision (Bin Arrow τ1 τ2) (Bin Arrow τ3 τ4)) as [C | nC] eqn:eq.
+    2: { exfalso. apply nC. by constructor. }
+    rewrite /cast. dependent destruction C. simpl.
+    f_equiv.
+    - rewrite /cast'.
+      destruct (consistency_decision τ3 τ1) as [C' | nC'] eqn:eq'; [| ].
+      2:{ exfalso. apply nC'. by apply consistency_sym. }
+      rewrite /cast. apply cast_pre_sym.
+    - rewrite /cast'.
+      destruct (consistency_decision τ2 τ4) as [C' | nC'] eqn:eq'; [| ].
+      2:{ exfalso. by apply nC'. }
+      rewrite /cast. apply cast_pre_const_rw.
+  Qed.
+
+  Lemma cast_product_rw ℓ τ1 τ2 τ3 τ4 (H13 : consistency τ1 τ3) (H24: consistency τ2 τ4) :
+    cast' ℓ (Bin Product τ1 τ2) (Bin Product τ3 τ4) =
+    bimap_prod ν (cast' ℓ τ1 τ3) (cast' ℓ τ2 τ4).
+  Proof.
+    rewrite /(cast' ℓ (Bin Product τ1 τ2) (Bin Product τ3 τ4)).
+    destruct (consistency_decision (Bin Product τ1 τ2) (Bin Product τ3 τ4)) as [C | nC] eqn:eq.
+    2: { exfalso. apply nC. by constructor. }
+    rewrite /cast. dependent destruction C. simpl.
+    f_equiv.
+    - rewrite /cast'.
+      destruct (consistency_decision τ1 τ3) as [C' | nC'] eqn:eq'; [| ].
+      2:{ exfalso. apply nC'. by apply consistency_sym. }
+      rewrite /cast. apply cast_pre_const_rw.
+    - rewrite /cast'.
+      destruct (consistency_decision τ2 τ4) as [C' | nC'] eqn:eq'; [| ].
+      2:{ exfalso. by apply nC'. }
+      rewrite /cast. apply cast_pre_const_rw.
+  Qed.
+
+  Lemma cast_sum_rw ℓ τ1 τ2 τ3 τ4 (H13 : consistency τ1 τ3) (H24: consistency τ2 τ4) :
+    cast' ℓ (Bin Sum τ1 τ2) (Bin Sum τ3 τ4) =
+    bimap_sum ν (cast' ℓ τ1 τ3) (cast' ℓ τ2 τ4).
+  Proof.
+    rewrite /(cast' ℓ (Bin Sum τ1 τ2) (Bin Sum τ3 τ4)).
+    destruct (consistency_decision (Bin Sum τ1 τ2) (Bin Sum τ3 τ4)) as [C | nC] eqn:eq.
+    2: { exfalso. apply nC. by constructor. }
+    rewrite /cast. dependent destruction C. simpl.
+    f_equiv.
+    - rewrite /cast'.
+      destruct (consistency_decision τ1 τ3) as [C' | nC'] eqn:eq'; [| ].
+      2:{ exfalso. apply nC'. by apply consistency_sym. }
+      rewrite /cast. apply cast_pre_const_rw.
+    - rewrite /cast'.
+      destruct (consistency_decision τ2 τ4) as [C' | nC'] eqn:eq'; [| ].
+      2:{ exfalso. by apply nC'. }
+      rewrite /cast. apply cast_pre_const_rw.
+  Qed.
+
+  Lemma cast_GU_rw ℓ G :
+    cast' ℓ (types.of_shape G) Unknown = Id.
+  Proof.
+    rewrite /cast' /cast.
+    destruct (consistency_decision (types.of_shape G) Unknown) as [C | nC] eqn:eq.
+    dependent destruction C; destruct G; (try destruct bin); simpl; try done; by repeat rewrite decide_True; auto.
+    exfalso. apply nC. destruct G; constructor.
+  Qed.
+
+  Lemma cast_factor_up_rw ℓ τ G :
+    to_ground τ = None → closed_ground τ = Some G →
+    cast' ℓ τ Unknown = comp Normal (cast' ℓ τ (types.of_shape G)) (cast' ℓ (types.of_shape G) Unknown).
+  Proof.
+    intros.
+    rewrite /(cast' ℓ τ Unknown).
+    destruct (consistency_decision τ Unknown) as [C | nC] eqn:eq. 2:{ exfalso. apply nC. constructor. }
+    rewrite /cast /cast_pre. dependent destruction C; simpl. 2:{ inversion H0. }
+    destruct τ; simplify_eq. simpl.
+    destruct (decide (τ1 = Unknown ∧ τ2 = Unknown)) as [[ -> -> ] | neq]. repeat rewrite /= decide_True in H; auto. inversion H.
+    assert (G = S_Bin bin) as ->. { simpl in H0. by destruct τ1; destruct τ2; simplify_eq. }
+    rewrite cast_GU_rw. asimpl. destruct bin.
+    - rewrite cast_arrow_rw; auto; try constructor.
+      by repeat rewrite -cast_downwards_rw; repeat rewrite -cast_upwards_rw.
+    - rewrite cast_sum_rw; auto; try constructor.
+      by repeat rewrite -cast_downwards_rw; repeat rewrite -cast_upwards_rw.
+    - rewrite cast_product_rw; auto; try constructor.
+      by repeat rewrite -cast_downwards_rw; repeat rewrite -cast_upwards_rw.
+  Qed.
+
+  Lemma cast_factor_down_rw ℓ τ G :
+    to_ground τ = None → closed_ground τ = Some G →
+    cast' ℓ Unknown τ = comp Normal (cast' ℓ Unknown (types.of_shape G)) (cast' ℓ (types.of_shape G) τ).
+  Proof.
+    intros.
+    rewrite /(cast' ℓ Unknown τ).
+    destruct (consistency_decision Unknown τ) as [C | nC] eqn:eq. 2:{ exfalso. apply nC. constructor. }
+    rewrite /cast /cast_pre. dependent destruction C; simpl. destruct G; inversion H0.
+    destruct τ; simplify_eq. simpl.
+    destruct (decide (τ1 = Unknown ∧ τ2 = Unknown)) as [[ -> -> ] | neq]. repeat rewrite /= decide_True in H; auto. inversion H.
+    assert (G = S_Bin bin) as ->. { simpl in H0. by destruct τ1; destruct τ2; simplify_eq. }
+    destruct bin.
+    - rewrite cast_downwards_rw /=. repeat rewrite decide_True; auto.
+      rewrite cast_arrow_rw; auto; try constructor.
+      repeat rewrite -cast_downwards_rw; repeat rewrite -cast_upwards_rw.
+      repeat rewrite cast'_closed. asimpl.
+      repeat rewrite -cast_downwards_rw; repeat rewrite -cast_upwards_rw.
+      repeat rewrite cast'_closed. auto.
+    - rewrite cast_downwards_rw /=. repeat rewrite decide_True; auto.
+      rewrite cast_sum_rw; auto; try constructor.
+    - rewrite cast_downwards_rw /=. repeat rewrite decide_True; auto.
+      rewrite cast_product_rw; auto; try constructor.
+  Qed.
+
 End casts_alt.
+
+(* From main.dyn_lang Require Import lemmas tactics. *)
+
+(* Section lemmas. *)
+
+(*   Context {ν : label} {Hν : NeverOccurs ν}. *)
+
+(*   Lemma rtc_step_ne_step e e' : rtc step_ne e e' → rtc step e e'. *)
+(*   Proof. induction 1. constructor. eapply rtc_l. by apply step_ne_step. auto. Qed. *)
+
+(*   Ltac take_step' := *)
+(*         (eapply rtc_l; first apply step_ne_step; first step_solver); asimpl. *)
+
+(*   Lemma error_faulty e ℓ : *)
+(*       faulty e ℓ → rtc step e (Error ℓ). *)
+(*   Proof. *)
+(*     intros. destruct H as (K & e_h & -> & [Hf | ->]). *)
+(*     - eapply (rtc_l _ _ (fill K (Error ℓ))). apply S_Normal. by apply H_error. *)
+(*       destruct K; econstructor; eauto. apply S_Error; auto. apply rtc_refl. *)
+(*     - destruct K; econstructor; eauto. apply S_Error; auto. apply rtc_refl. *)
+(*   Qed. *)
+
+(* End lemmas. *)
