theories/cast_calc/lemmas.v
@@ -1,0 +1,197 @@
+From main.prelude Require Import imports base_lang tactics.
+From main.cast_calc Require Import definition.
+
+Lemma fill_app K K' e : fill (K ++ K') e = fill K (fill K' e).
+Proof.
+  generalize dependent e.
+  induction K; auto.
+  intro e. simpl. by rewrite IHK.
+Qed.
+
+Instance fill_item_inj Ki : Inj (=) (=) (fill_item Ki).
+Proof. destruct Ki; intros ???; simplify_eq/=; auto with f_equal. Qed.
+
+Lemma head_step_not_val e1 e2 :
+  head_step e1 e2 → to_val e1 = None.
+Proof.
+  destruct 1; destruct Hs; auto; (try done);
+    simplify_option_eq; (try done).
+  destruct (_ : shape); [ | destruct (_ : bin_const) ]; simplify_option_eq; auto.
+  - destruct G1. destruct b; simplify_option_eq; destruct G2; simplify_option_eq; try done;
+    destruct bin; auto; by exfalso.
+    destruct bin; simplify_option_eq; destruct G2; simplify_option_eq; (try destruct bin); done.
+  - destruct τ; (try destruct bin); auto.
+  - destruct τ; (try destruct bin); auto. destruct τ1, τ2; auto. by exfalso.
+Qed.
+
+Lemma fill_item_not_val Ki e :
+  to_val e = None → to_val (fill_item Ki e) = None.
+Proof. intros. by destruct Ki; simpl; (try rewrite to_of_val); auto; simplify_option_eq. Qed.
+
+Lemma fill_not_val K :
+  ∀ e, to_val e = None → to_val (fill K e) = None.
+Proof.
+  induction K as [|Ki K] using rev_ind ; auto. intros.
+  rewrite /fill foldr_snoc /=. fold (fill K (fill_item Ki e)).
+  apply IHK. by apply fill_item_not_val.
+Qed.
+
+Lemma step_no_val e1 e2 :
+  step e1 e2 → to_val e1 = None.
+Proof.
+  destruct 1; auto. apply fill_not_val.
+  by eapply head_step_not_val. by apply fill_not_val.
+Qed.
+
+Instance fill_inj K : Inj (=) (=) (fill K).
+Proof.
+  induction K as [| Ki K IH]; rewrite /Inj; naive_solver.
+Qed.
+
+Instance of_val_inj : Inj (=) (=) of_val.
+Proof. by intros ?? Hv; apply (inj Some); rewrite -!to_of_val Hv. Qed.
+
+Instance Var_Inj : Inj eq eq Var. intros x1 x2 eq. by inversion eq. Qed.
+
+Lemma fill_item_no_val_inj Ki1 Ki2 e1 e2 :
+  to_val e1 = None → to_val e2 = None →
+  fill_item Ki1 e1 = fill_item Ki2 e2 → Ki1 = Ki2.
+Proof.
+  destruct Ki1, Ki2; intros; try discriminate; simplify_eq;
+  repeat match goal with
+          | H : to_val (of_val _) = None |- _ => by rewrite to_of_val in H
+          end; auto.
+Qed.
+
+Lemma pure_step_by_val' K K' e1 e1' ℓ :
+  fill K e1 = fill K' e1' →
+  to_val e1 = None →
+  (e1' = Error ℓ) →
+  ∃ K'', K' = K ++ K''.
+Proof.
+  intros Hfill Hred ->.
+  revert K' Hfill.
+  induction K as [|Ki K IH]=> /= K' Hfill; eauto using app_nil_l.
+  destruct K' as [|Ki' K']; simplify_eq/=.
+  { assert (H := (fill_not_val K _ Hred)).
+    destruct Ki; inversion Hfill. }
+  assert (Ki = Ki') as ->.
+  { eapply fill_item_no_val_inj, Hfill.
+    by apply fill_not_val. apply fill_not_val. auto.
+  }
+  simplify_eq. destruct (IH K') as [K'' ->]; auto. by exists K''.
+Qed.
+
+Lemma pure_head_ctx_step_val Ki e e2 :
+  head_step (fill_item Ki e) e2 → is_Some (to_val e).
+Proof.
+  intros H. invclear H; invclear Hs; simplify_eq; destruct Ki; simplify_option_eq; try by eexists; eauto.
+  destruct G; (try destruct bin); simplify_option_eq; eexists; eauto.
+  destruct G1; (try destruct bin); simplify_option_eq; eexists; eauto.
+  destruct G; (try destruct bin); simplify_option_eq; eexists; eauto.
+Qed.
+
+Lemma fill_item_val Ki e :
+  is_Some (to_val (fill_item Ki e)) → is_Some (to_val e).
+Proof. intros [v ?]. destruct Ki; simplify_option_eq; eauto. Qed.
+
+Lemma fill_val K e : is_Some (to_val (fill K e)) → is_Some (to_val e).
+Proof.
+  revert e. induction K as [|Ki K IHK] using rev_ind; first by simpl.
+  intros e pev. apply fill_item_val with (Ki := Ki).
+  apply IHK. rewrite fill_app in pev. by simpl.
+Qed.
+
+Lemma pure_step_by_val K K' e1 e1' e2 :
+  fill K e1 = fill K' e1' →
+  to_val e1 = None →
+  head_step e1' e2 →
+  ∃ K'', K' = K ++ K''.
+Proof.
+  intros Hfill Hred Hstep.
+  revert K' Hfill.
+  induction K as [|Ki K IH]=> /= K' Hfill; eauto using app_nil_l.
+  destruct K' as [|Ki' K']; simplify_eq/=.
+  { apply pure_head_ctx_step_val in Hstep.
+    apply fill_val in Hstep. by apply not_eq_None_Some in Hstep. }
+  (* change (fill_item ?Ki (fill ?K ?e)) with (fill (Ki :: K) e) in Hfill. *)
+  assert (Ki = Ki') as ->.
+  { eapply fill_item_no_val_inj, Hfill.
+    by apply fill_not_val. apply fill_not_val.  eauto using head_step_not_val. }
+  simplify_eq. destruct (IH K') as [K'' ->]; auto. by exists K''.
+Qed.
+
+
+Lemma head_step_det e e1 e2 : head_step e e1 → head_step e e2 → e1 = e2.
+Proof.
+  intros H1 H2.
+  invclear H1.
+  - invclear H2.
+    + try by invclear Hs; invclear Hs0.
+    + exfalso.
+      try by invclear Hs; invclear Hs0.
+  - invclear H2.
+    + exfalso. try by invclear Hs; invclear Hs0.
+    + invclear Hs; invclear Hs0; try done.
+      * destruct G; invclear H1.
+      * destruct G2; invclear H1.
+      * destruct G; invclear H3.
+      * destruct G1; destruct G2; simplify_eq.
+      * destruct G; destruct G0; simplify_eq.
+      * destruct G2; invclear H4.
+      * destruct G; destruct G1; destruct G2; simplify_eq.
+      * destruct G2; invclear H7.
+      * destruct G; destruct G0; auto; try by destruct bin; destruct b; simplify_eq.
+        by destruct bin; destruct bin0; simplify_eq.
+      * destruct G0; inversion H0. repeat rewrite decide_True in H3; auto.
+        simplify_eq.
+      * destruct G2; inversion H0. repeat rewrite decide_True in H3; auto.
+        simplify_eq.
+Qed.
+
+Lemma fill_item_Error_head_step_false Ki ℓ eh' : head_step (fill_item Ki (Error ℓ)) eh' → False.
+Proof. intros Hs. invclear Hs; invclear Hs0; destruct Ki; simplify_eq; try by invclear H. Qed.
+
+Lemma fill_Error_head_step_false K ℓ eh' : head_step (fill K (Error ℓ)) eh' → False.
+Proof.
+  destruct K as [| Ki K].
+  intros Hs. invclear Hs; invclear Hs0; simplify_eq.
+  simpl. intros abs.
+  destruct (pure_head_ctx_step_val _ _ _ abs) as [v abs'].
+  rewrite (fill_not_val K) in abs'; simplify_eq. auto.
+Qed.
+
+Lemma step_det e e1 e2 : step e e1 → step e e2 → e1 = e2.
+Proof.
+  intros H1 H2.
+  invclear H1; invclear H2.
+  - assert (K = K0) as <-.
+    { destruct (pure_step_by_val K0 K e_h0 e_h e_h' H0 ltac:(by eapply head_step_not_val) ltac:(eauto)) as [Kred eq].
+      destruct (pure_step_by_val K K0 _ _ e_h'0 (eq_Symmetric _ _ H0) ltac:(by eapply head_step_not_val) ltac:(eauto)) as [Kred' eq'].
+      assert (H: length K = length ((K ++ Kred') ++ Kred)). by rewrite -eq' eq. rewrite -app_assoc app_length app_length in H.
+      destruct Kred'; [ | exfalso; simpl in *; lia ]. destruct Kred; [ | exfalso; simpl in *; lia ].
+      by rewrite app_nil_r in eq. }
+    f_equal. rewrite (fill_inj K _ _ H0) in HS0. by eapply head_step_det.
+  - exfalso.
+    destruct (pure_step_by_val' K K0 e_h (Error ℓ) ltac:(eauto) (eq_Symmetric _ _ H) ltac:(by eapply head_step_not_val)) as [Kred eq]; auto. simplify_eq.
+    rewrite fill_app in H.
+    assert (fill Kred (Error ℓ) = e_h). eapply fill_inj. apply H. simplify_eq.
+    by eapply fill_Error_head_step_false.
+  - exfalso.
+    destruct (pure_step_by_val' K0 K e_h (Error ℓ) ltac:(eauto) (H1) ltac:(by eapply head_step_not_val)) as [Kred eq]; auto. simplify_eq.
+    rewrite fill_app in H1.
+    assert (e_h = fill Kred (Error ℓ)). eapply fill_inj. apply H1. simplify_eq.
+    by eapply fill_Error_head_step_false.
+  - destruct (pure_step_by_val' K K0 (Error ℓ) (Error ℓ0) ℓ0 ltac:(eapply (eq_Symmetric _ _ H0)) ltac:(eauto) ltac:(eauto)) as [Kred eq].
+    destruct (pure_step_by_val' K0 K (Error ℓ0) (Error ℓ) ℓ H0 ltac:(eauto) ltac:(eauto)) as [Kred' eq'].
+
+    simplify_eq.
+    assert (length (Kred') = 0).
+    { assert (length K0 = length ((K0 ++ Kred') ++ Kred)). by rewrite -eq.
+      destruct Kred; destruct Kred';
+      repeat rewrite app_length /= in H2; auto; lia.
+    }
+    destruct Kred'; destruct Kred; simplify_eq. simpl in *.
+    rewrite app_nil_r in H0. by eapply fill_inj.
+    rewrite app_nil_r in H0. by eapply fill_inj.
+Qed.
