theories/cast_calc/simul/equiv.v
@@ -1,0 +1,69 @@
+From main Require Import imports prelude.autosubst prelude.tactics.
+(* From main.grad_lang Require Import types definition. *)
+From main.grad_lang Require Import types.
+From main.cast_calc Require Import definition typing lemmas.
+From main.cast_calc.simul Require Import invariant prog_pres.
+From main.dyn_lang Require Import definition casts lib lemmas tactics.
+
+Section universal.
+
+  Context {ν : label} {Hν : NeverOccurs ν}.
+
+  Lemma universal e τ (He : typed [] e τ) e' (HI : Invariant e e') :
+    ∀ n en, nsteps cc_step n e en →
+            typed [] en τ ∧ ∃ m em', n ≤ m ∧ nsteps dn_step m e' em' ∧ Invariant_EC en em'.
+  Proof.
+    intros n. induction n; intros.
+    - invclear H. split; auto. exists 0, e'. repeat split; eauto; repeat constructor; auto.
+    - rename en into eSn. destruct (nsteps_inv_r _ _ _ H) as (en & Hn & Hs).
+      specialize (IHn en Hn) as (Hτen & m & em & Hnm & Hms & HIm).
+      split. by eapply preservation.
+      destruct (left_step_Invariant_EC _ _ Hτen _ HIm _ Hs) as (efm & Hemefm & HIf).
+      destruct (iffLR (tc_nsteps _ _) Hemefm) as (k & Hk & Hksteps).
+      exists (m + k), efm. split; [ lia |]. split; auto.
+      by eapply nsteps_trans.
+  Qed.
+
+End universal.
+
+Section simulation.
+
+  Context {ν : label} {Hν : NeverOccurs ν}.
+
+  Lemma ref_val e τ (He : typed [] e τ) v :
+    rtc cc_step e (cc_of_val v) →
+    ∃ v', rtc step ⌜e⌝ (of_val v') ∧ Invariant (cc_of_val v) (of_val v').
+  Proof.
+    intros H. destruct (iffLR (rtc_nsteps _ _) H) as (k & Hksteps).
+    destruct (universal e τ He (simul_expr e) (simul_expr_Invariant _ e _ He) k (cc_of_val v) Hksteps) as (Hτv & m & ev & _ & Hdmsteps & HIvev).
+    invclear HIvev.
+    2:{ exfalso. assert (Hmm := cc_to_of_val v). rewrite -H1 in Hmm.
+        by rewrite (cast_calc.lemmas.fill_not_val K) in Hmm. }
+    destruct (left_val_Invariant _ _ HI _ Hτv v (cc_to_of_val v)) as (v' & Hsteps & HIvv').
+    exists v'. split; eauto. eapply rtc_transitive. by eapply rtc_nsteps_2.
+    eapply (rtc_congruence id); [| apply Hsteps ]. by apply step_ne_step.
+  Qed.
+
+  Lemma ref_div e τ (He : typed [] e τ) :
+    (∀ n, ∃ e', nsteps cc_step n e e') →
+    (∀ n, ∃ e', nsteps step n ⌜e⌝ e').
+  Proof.
+    intros H n. destruct (H n) as (e' & Hnsteps).
+    destruct (universal e τ He (simul_expr e) (simul_expr_Invariant _ e _ He) n _ Hnsteps) as (Hτv & m & ev & Hm & Hdmsteps & HIvev).
+    assert (∃ k, n + k = m) as [k eq]. exists (m - n). lia.
+    rewrite -eq in Hdmsteps.
+    destruct (nsteps_add_inv _ _ _ _ Hdmsteps) as (ei & Hstepsi & Hstepsf).
+    exists ei. auto.
+  Qed.
+
+  Lemma ref_error e τ (He : typed [] e τ) ℓ :
+    (rtc cc_step e (cc_Error ℓ)) →
+    (rtc step ⌜e⌝ (Error ℓ)).
+  Proof.
+    intros H. destruct (iffLR (rtc_nsteps _ _) H) as (k & Hksteps).
+    destruct (universal e τ He (simul_expr e) (simul_expr_Invariant _ e _ He) k _ Hksteps) as (Hτv & m & t & _ & Hdmsteps & HIvev).
+    invclear HIvev. 2:{ exfalso. destruct K as [|Ki K]; invclear H1. destruct Ki; invclear H2. }
+    destruct t; invclear HI. apply rtc_nsteps. by eexists.
+  Qed.
+
+End simulation.
