theories/logrel/examples/tautology.v
@@ -1,0 +1,154 @@
+From main.prelude Require Import imports autosubst big_op_three.
+From main.grad_lang Require Import types.
+From main.dyn_lang Require Import definition lemmas lib labels tactics.
+From main.logrel.lib Require Import weakestpre rfn small_helpers recursion.
+From main.logrel Require Import definition.
+
+From iris.si_logic Require Export bi.
+From iris.proofmode Require Import tactics.
+(* From iris.proofmode Require Import base proofmode classes. *)
+
+Section tautology_example.
+
+  Context {ν : label} {Hν : NeverOccurs ν}.
+
+  (* "David Turner’s tautology program" *)
+  (* Courtesy to reviewer A *)
+
+  Definition isZero (e : expr) : expr :=
+     BinOp ν EqOp 0 e.
+
+  Definition MinusOne (e : expr) : expr :=
+     BinOp ν MinusOp e 1.
+
+  Definition And (e1 e2 : expr) : expr :=
+     If ν e1 (If ν e2 true false) false.
+
+  Definition tautV : val :=
+    RecV (*n*) (*f*) (
+     If ν (isZero (Var 0(*n*)))
+     (* then *) (Lam (Var 0))
+     (* esle *) (Lam (*g*) (And ((Var 2(*r*)) (MinusOne (Var 1(*n*))) ((Var 0(*g*)) true))
+                                ((Var 2(*r*)) (MinusOne (Var 1(*n*))) ((Var 0(*g*)) false))))
+      ).
+  (* taut 0 g  =  g *)
+  (* taut n g  =  taut (n-1) (g false) && taut (n-1) (g true) *)
+
+
+  Notation taut := (of_val tautV).
+
+  Ltac rfn_steps :=
+    asimpl; (rfn_l_s; asimpl); (rfn_r_s; asimpl).
+
+  Fixpoint dom_taut (n : nat) : type :=
+    match n with
+    | O => Base Bool
+    | S n => Bin Arrow (Base Bool) (dom_taut n)
+    end.
+
+  Definition type_taut (n : nat) : type := Bin Arrow (dom_taut n) (Base Bool).
+
+  Lemma taut_closed : Closed taut.
+  Proof. intros σ. rewrite /taut Rec_subst. by asimpl. Qed.
+
+  Lemma taut_sem_typed (n : nat) : sem_typed [] (taut n) (type_taut n).
+  Proof.
+    split. 2: { intros σ. rewrite /taut. asimpl. rewrite Rec_subst. by asimpl. }
+    induction n; rewrite /taut.
+    - iIntros (Δ HΔ vs vs') "_". asimpl. rewrite /type_taut /=.
+      do 2 rewrite Rec_subst. asimpl.
+      iApply rfn_lr_Rec_App; auto. asimpl.
+      rfn_steps. repeat rewrite bool_decide_true; auto. rfn_steps. rfn_val.
+      repeat iNext. iIntros (v v') "#Hvv'". rfn_val.
+    - iIntros (Δ HΔ vs vs') "#H". asimpl.
+      do 2 rewrite Rec_subst. asimpl.
+      iApply rfn_lr_Rec_App; auto. asimpl.
+      rfn_steps. repeat rewrite bool_decide_false; auto. repeat rfn_steps.
+      repeat iNext. rfn_val.
+      iIntros (g g') "#Hgg'".
+
+      repeat rfn_steps.
+      assert ((S n - 1%nat)%Z = n) as -> by by lia.
+
+      specialize (IHn Δ HΔ vs vs').
+      iDestruct (IHn with "H") as "HHH".
+
+      change ((Rec
+                  (If ν (BinOp ν EqOp 0 (ids 0))
+                     (Lam (ids 0))
+                     (Lam
+                        (If ν
+                           (App ν
+                              (App ν (ids 2)
+                                 (BinOp ν MinusOp (ids 1) 1))
+                              (App ν (ids 0) true))
+                           (If ν
+                              (App ν
+                                 (App ν (ids 2)
+                                    (BinOp ν MinusOp (ids 1) 1))
+                                 (App ν (ids 0) false)) true false)
+                           false)))) ) with (taut).
+      repeat rewrite /= taut_closed.
+      rfn_bind_pp. iApply "HHH".
+      iNext.
+
+      iIntros (k k') "#Hkk'".
+      dvals g g'. rfn_bind_pp. rfn_steps. rw_of_val. by iApply "Hgg'".
+
+      iIntros (l l') "#Hll'".
+
+      dvals k k'. rfn_steps. rfn_bind. by iApply "Hkk'".
+
+      iNext. iIntros (b b') "#Hbb'".
+      dvals b b'. iDestruct "Hbb'" as "<-". destruct b; repeat rfn_steps; [| rfn_val].
+      assert ((S n - 1%nat)%Z = n) as -> by by lia.
+      rfn_bind_pp. iApply "HHH".
+      repeat iNext. iIntros (m m') "#Hmm'".
+      dvals m m'. rfn_steps. rfn_bind. rw_of_val. iApply "Hgg'". auto.
+      iNext. iIntros (o o') "#Hoo'". rfn_steps. iNext.
+      rfn_bind. by iApply "Hmm'".
+      iIntros (b b') "Hbb'". dvals b b'. iDestruct "Hbb'" as "<-".
+      rfn_steps. destruct b; rfn_val.
+  Qed.
+
+
+  (* just as illustration; tautology function is well typed in coq *)
+
+  Fixpoint dom_taut_coq (n : nat) : Type :=
+    match n with
+    | O => bool
+    | S n => bool → (dom_taut_coq n)
+    end.
+
+  Definition type_taut_coq (n : nat) : Type :=
+    dom_taut_coq n → bool.
+
+  Compute (type_taut_coq 3).
+
+  Fixpoint taut_coq (n : nat) : (type_taut_coq n) :=
+    match n with
+    | O => fun g => g
+    | S n => fun g => (taut_coq n (g false)) && (taut_coq n (g true))
+    end.
+
+   Fixpoint taut_coq (n : nat) (g : dom_taut_coq n) : bool :=
+    match n with
+    | O => g
+    | S n => (taut_coq n (g false)) && (taut_coq n (g true))
+    end.
+
+  (* taut 0 g  =  g *)
+  (* taut n g  =  taut (n-1) (g false) && taut (n-1) (g true) *)
+
+
+
+    RecV (*n*) (*f*) (
+     If ν (isZero (Var 0(*n*)))
+     (* then *) (Lam (Var 0))
+     (* esle *) (Lam (*g*) (And ((Var 2(*r*)) (MinusOne (Var 1(*n*))) ((Var 0(*g*)) true))
+                                ((Var 2(*r*)) (MinusOne (Var 1(*n*))) ((Var 0(*g*)) false))))
+      ).
+
+
+
+End tautology_example.
