theories/logrel/lib/recursion.v
@@ -1,0 +1,113 @@
+From main.prelude Require Import imports autosubst big_op_three.
+From main.grad_lang Require Import types.
+From main.dyn_lang Require Import definition lemmas lib labels tactics.
+From main.logrel.lib Require Import weakestpre rfn small_helpers.
+From main.logrel Require Import definition.
+
+From iris.si_logic Require Export bi.
+From iris.proofmode Require Import tactics.
+(* From iris.proofmode Require Import base proofmode classes. *)
+
+Section recursion.
+
+  Context {ν : label} {Hν : NeverOccurs ν}.
+
+  Coercion LitInt : Z >-> base_lit.
+  Coercion LitBool : bool >-> base_lit.
+  Coercion Lit : base_lit >-> expr.
+  Coercion AppAn : expr >-> Funclass.
+  Coercion Var : var >-> expr.
+
+  Definition FixArrow (f : expr) : expr :=
+    (Lam ((f.[ren (+1)]) (Lam ((Var 1) (Var 1) (Var 0)))))
+      ((Lam (f.[ren (+1)] (Lam ((Var 1) (Var 1) (Var 0)))))).
+
+  Lemma FixArrow_subst e σ : (FixArrow e).[σ] = FixArrow e.[σ].
+  Proof. rewrite /FixArrow. by asimpl. Qed.
+
+  Lemma FixArrow_eval f : step_ne (FixArrow f) (f (Lam ((FixArrow f).[ren (+1)] (Var 0)))).
+  Proof.
+    eassert (step_ne (FixArrow f) _). rewrite /FixArrow. step_solver.
+    asimpl in H. rewrite /FixArrow. by asimpl.
+  Qed.
+
+  Definition RecV' (e : {bind 2 of expr}) : val :=
+    LamV ((FixArrow (Lam (Lam e))).[ren (+1)] (Var 0)).
+  (* we'll leave RecV for sealed one *)
+
+  Definition Rec' e := of_val (RecV' e).
+
+  Lemma Rec'_subst (e : {bind 2 of expr}) σ : (Rec' e).[σ] = Rec' (e.[ids 0 .: ids 1 .: σ >> ren (+2)]).
+  Proof. by asimpl. Qed.
+
+  Global Opaque FixArrow.
+
+  Lemma App_Rec'_eval e1 v2 :
+    nsteps step_ne 4 ((Rec' e1) (of_val v2)) e1.[(of_val v2), (Rec' e1)/].
+  Proof.
+    intros.
+    eapply nsteps_l. rewrite /Rec'. step_solver. asimpl. rewrite FixArrow_subst.
+    change 3 with (1 + 2).
+    eapply nsteps_trans.
+    assert (Hf := FixArrow_eval (Lam (Lam e1))).
+    apply nsteps_once. rw_fill. eapply fill_step. apply Hf.
+    eapply nsteps_l. step_solver. asimpl.
+    eapply nsteps_l. step_solver. asimpl.
+    rewrite FixArrow_subst. asimpl.
+    constructor.
+  Qed.
+
+  (* this does not work sadly *)
+  (* Global Opaque Rec. *)
+  (* Global Opaque RecV. *)
+
+  (* Definition Rec_aux : seal Rec. Proof. by eexists. Qed. *)
+  (* Definition Rec' := Rec_aux.(unseal). *)
+  (* Lemma Rec_unseal : Rec = Rec'. *)
+  (* Proof. by rewrite -Rec_aux.(seal_eq) /=. Qed. *)
+
+  Definition RecV_aux : seal RecV'. Proof. by eexists. Qed.
+  Definition RecV := RecV_aux.(unseal).
+  Lemma RecV_unseal : RecV = RecV'.
+  Proof. by rewrite -RecV_aux.(seal_eq) /=. Qed.
+  Lemma RecV_seal : RecV' = RecV.
+  Proof. by rewrite -RecV_unseal. Qed.
+
+  Notation Rec e := (of_val (RecV e)).
+
+  Lemma wp_Rec L e e' v' (He' : to_val e' = Some v') Φ :
+    ▷ wp Φ L e.[e', (Rec e)/] ⊢ wp Φ L (Rec e e').
+  Proof.
+    iIntros.
+    rewrite -(of_to_val _ _ He'). iApply wp_nsteps.
+    rewrite RecV_unseal.
+    change (of_val (RecV' e)) with (Rec' e). apply App_Rec'_eval.
+    change (Rec' e) with (of_val (RecV' e)). rewrite RecV_seal. auto.
+  Qed.
+
+  Lemma Rec_subst (e : {bind 2 of expr}) σ : (Rec e).[σ] = Rec (e.[ids 0 .: ids 1 .: σ >> ren (+2)]).
+  Proof. rewrite RecV_unseal. by rewrite Rec'_subst. Qed.
+
+  Lemma App_Rec_eval e1 v2 :
+    nsteps step_ne 4 ((Rec e1) (of_val v2)) e1.[(of_val v2), (Rec e1)/].
+  Proof. rewrite RecV_unseal. apply App_Rec'_eval. Qed.
+
+  Lemma rfn_r_Rec_App L t e e' v' (He' : to_val e' = Some v') Φ :
+    rfn Φ L t e.[e', (Rec e)/] ⊢ rfn Φ L t (Rec e e').
+  Proof.
+    rewrite -(of_to_val _ _ He').
+    iIntros. iApply rfn_steps_r. eapply rtc_nsteps_2. eapply App_Rec_eval. auto.
+  Qed.
+
+  Lemma rfn_lr_Rec_App L t t' w' (Ht' : to_val t' = Some w') e e' v' (He' : to_val e' = Some v') Φ :
+    ▷ rfn Φ L t.[t', (Rec t)/] e.[e', (Rec e)/] ⊢ rfn Φ L (Rec t t') (Rec e e').
+  Proof.
+    rewrite -(of_to_val _ _ Ht') -(of_to_val _ _ He').
+    iIntros. iApply rfn_steps_r. eapply rtc_nsteps_2. eapply App_Rec_eval.
+    iApply wp_impl. iApply wp_Rec. by rewrite to_of_val. auto.
+    auto. auto.
+  Qed.
+
+End recursion.
+
+Notation Rec e := (of_val (RecV e)).
