theories/prelude/tactics.v
@@ -1,0 +1,4 @@
+From stdpp Require Export prelude.
+From iris Require Export prelude.
+
+Ltac invclear H := inversion H; simplify_eq; clear H.
